lemmas.v
@@ -1,0 +1,58 @@
+Require Import List.
+Import ListNotations.
+Require Import Arith.
+Require Import Logic.
+Require Import Psatz.
+Require Import Bool.
+Require Import definitions.
+
+
+Lemma not_lt_0 : forall (n : nat), ~(n < 0).
+  lia.
+Qed.
+
+Lemma not_lt_eq : forall (n : nat) (m : nat), n < m -> Nat.eqb n m = false.
+Proof.
+  intro. induction n.
+  intros.
+  simpl.
+  inversion H.
+  trivial. trivial.
+  intros.
+  destruct m.
+  trivial.
+  simpl.
+  apply IHn.
+  apply le_S_n. trivial.
+Qed.
+
+
+Lemma minus_0_le : forall (n : nat) (m : nat), n-m = 0 -> n <= m.
+Proof.
+  lia.
+Qed.
+
+Lemma lt_add : forall (i : nat) (n : nat) (m : nat), i+n < i+m -> n < m.
+Proof.
+  lia.
+Qed.
+
+Lemma sub_0 : forall n, n-0 = n.
+Proof.
+  lia.
+Qed.
+
+
+Lemma not_le : forall n m, ~ (n < m) -> m <= n.
+Proof.
+  lia.
+Qed.
+Lemma NotLt : forall n m, ~(n <= m) -> m < n.
+  lia.
+Qed.
+
+Lemma sub_ineq : forall a b c,
+  a < b + c -> a >= b -> a - b < c.
+Proof.
+  lia.
+Qed.
